start Add1sp1 proof

code/mpfr/MPFR.Add1.Spec.fst
@@ -11,23 +11,20 @@ open MPFR.Maths
 
 (* Useful functions when adding two MPFR numbers with same precision
  * and the exponent of the first one is greater than that of the second one *)
-val add_sp_ge_limb: a:mpfr_reg_fp -> b:mpfr_reg_fp -> Pure nat
-    (requires (a.sign = b.sign /\ a.prec = b.prec /\ a.exp >= b.exp))
-    (ensures  (fun rm -> rm * a.sign = (eval a +. eval b).significand /\
-                      rm % pow2 (a.len - a.prec) = 0))
-    
+val add_sp_ge_limb: a:mpfr_reg_fp ->
+    b:mpfr_reg_fp{a.prec = b.prec /\ a.exp >= b.exp} ->
+    Tot (rm:nat{rm = (eval_abs a +. eval_abs b).significand /\ rm % pow2 (a.len - a.prec) = 0})
+
 let add_sp_ge_limb a b =
-    lemma_distr_add_left a.sign (a.limb * pow2 (a.exp - b.exp)) (b.limb * pow2 0);
-    //! assert((a.limb * pow2 (a.exp - b.exp) + b.limb) * a.sign = (eval a +. eval b).significand);
-    lemma_mul_mod a.limb (pow2 (a.exp - b.exp)) (pow2 (a.len - a.prec));
+    assert((a.limb * pow2 (a.exp - b.exp) + b.limb) = (eval_abs a +. eval_abs b).significand);
+    lemma_mul_mod_zero a.limb (pow2 (a.exp - b.exp)) (pow2 (a.len - a.prec));
     lemma_mod_distr_zero (a.limb * pow2 (a.exp - b.exp)) b.limb (pow2 (a.len - a.prec));
     //! assert((a.limb * pow2 (a.exp - b.exp) + b.limb) % pow2 (a.len - a.prec) = 0);
     a.limb * pow2 (a.exp - b.exp) + b.limb
 
-val add_sp_ge_len: a:mpfr_reg_fp -> b:mpfr_reg_fp -> Pure pos
-    (requires (a.sign = b.sign /\ a.prec = b.prec /\ a.exp >= b.exp))
-    (ensures  (fun rl -> add_sp_ge_limb a b >= pow2 (rl - 1) /\
-                      add_sp_ge_limb a b < pow2 rl))
+val add_sp_ge_len: a:mpfr_reg_fp -> 
+    b:mpfr_reg_fp{a.prec = b.prec /\ a.exp >= b.exp} ->
+    Tot (rl:pos{add_sp_ge_limb a b >= pow2 (rl - 1) /\ add_sp_ge_limb a b < pow2 rl})
 
 let add_sp_ge_len a b =
     let d = a.exp - b.exp in
@@ -45,24 +42,25 @@ let add_sp_ge_len a b =
 	a.len + d + 1
     end
 
-val add_sp_ge_exp: a:mpfr_reg_fp -> b:mpfr_reg_fp -> Pure int
-    (requires (a.sign = b.sign /\ a.prec = b.prec /\ a.exp >= b.exp))
-    (ensures  (fun rx -> rx - add_sp_ge_len a b = (eval a +. eval b).exponent))
+val add_sp_ge_exp: a:mpfr_reg_fp ->
+    b:mpfr_reg_fp{a.prec = b.prec /\ a.exp >= b.exp} ->
+    Tot (rx:int{rx - add_sp_ge_len a b = (eval a +. eval b).exponent})
 
 let add_sp_ge_exp a b =
     if add_sp_ge_limb a b < pow2 (a.len + a.exp - b.exp) then a.exp else a.exp + 1
     
-val add_sp_ge_prec: a:mpfr_reg_fp -> b:mpfr_reg_fp -> Pure pos
-    (requires (a.sign = b.sign /\ a.prec = b.prec /\ a.exp >= b.exp))
-    (ensures  (fun rp -> add_sp_ge_len a b - rp = a.len - a.prec))
+val add_sp_ge_prec: a:mpfr_reg_fp ->
+    b:mpfr_reg_fp{a.prec = b.prec /\ a.exp >= b.exp} ->
+    Tot (rp:pos{add_sp_ge_len a b - rp = a.len - a.prec})
     
 let add_sp_ge_prec a b = a.prec + add_sp_ge_len a b - a.len
 
 (* Addition for two MPFR numbers with same precision *)
-val add_sp: a:mpfr_reg_fp -> b:mpfr_reg_fp -> Pure normal_fp
-    (requires (a.sign = b.sign /\ a.prec = b.prec))
-    (ensures  (fun r -> eval a +. eval b =. eval r))
+val add_sp: a:mpfr_reg_fp ->
+    b:mpfr_reg_fp{a.prec = b.prec} ->
+    Tot (r:normal_fp{r.sign = a.sign /\ eval_abs a +. eval_abs b =. eval_abs r})
     
 let add_sp a b = 
+    let rs = a.sign in
     let a, b = if a.exp >= b.exp then a, b else b, a in
-    mk_normal a.sign (add_sp_ge_prec a b) (add_sp_ge_exp a b) (add_sp_ge_limb a b) (add_sp_ge_len a b) MPFR_NUM
+    mk_normal rs (add_sp_ge_prec a b) (add_sp_ge_exp a b) (add_sp_ge_limb a b) (add_sp_ge_len a b) MPFR_NUM
