code/mpfr/MPFR.Add1sp1.fst
@@ -9,15 +9,18 @@ open FStar.UInt64
 open FStar.Int.Cast
 open FStar.Mul
 open MPFR.Lib
+open MPFR.Lib.Spec
 open MPFR.Maths
 
 module I64 = FStar.Int64
 module I32 = FStar.Int32
 module U32 = FStar.UInt32
 module Spec = MPFR.Add1.Spec
+module RND  = MPFR.Round.Spec
 
-#set-options "--z3refresh --z3rlimit 20 --max_fuel 1 --initial_fuel 0 --max_ifuel 1 --initial_ifuel 0"
+#set-options "--z3refresh --z3rlimit 60 --max_fuel 1 --initial_fuel 0 --max_ifuel 1 --initial_ifuel 0"
 
+(* intermediate results *)
 private type mpfr_tmp_exp_t = x:mpfr_exp_t{I32.(x >=^ mpfr_EMIN /\ x <=^ mpfr_EMAX +^ 1l)}
 
 noeq type state = {
@@ -34,30 +37,211 @@ let mk_state sh bx rb sb = {
     sb = sb
 }
 
-(* TODO: remove abundent inputs *)
+(* lemmas and implementation for mpfr_add1sp1_gt_branch1 where
+ * b.exp > c.exp && d < sh *)
+let mpfr_add1sp1_gt_branch1_precond h a b c sh d mask =
+    mpfr_reg_struct_cond h b /\ mpfr_reg_struct_cond h c /\
+    U32.v a.mpfr_prec < U32.v gmp_NUMB_BITS - 1 /\
+    U32.v a.mpfr_prec = U32.v b.mpfr_prec /\
+    U32.v a.mpfr_prec = U32.v c.mpfr_prec /\
+    U32.v sh = U32.v gmp_NUMB_BITS - U32.v a.mpfr_prec /\
+    I32.v b.mpfr_exp > I32.v c.mpfr_exp /\
+    U32.v d = I32.v b.mpfr_exp - I32.v c.mpfr_exp /\
+    U32.v d < U32.v sh /\ v mask = pow2 (U32.v sh) - 1 /\
+    (let am = a.mpfr_d in
+    let bm = b.mpfr_d in
+    let cm = c.mpfr_d in
+    live h am /\ live h bm /\ live h cm /\
+    length am = 1 /\ length bm = 1 /\ length cm = 1)
+    
+val mpfr_add1sp1_gt_branch1_a0_bx_lemma:
+    h0:mem -> h1:mem ->
+    a:mpfr_struct -> b:mpfr_struct -> c:mpfr_struct ->
+    sh:mpfr_reg_prec_t -> d:u32 -> mask:mp_limb_t -> Lemma
+    (requires (mpfr_add1sp1_gt_branch1_precond h0 a b c sh d mask))
+    (ensures  (
+    let r = Spec.add_sp (as_reg_fp_ h0 b) (as_reg_fp_ h0 c) in
+    let bp = b.mpfr_d in
+    let cp = c.mpfr_d in
+    let bx = b.mpfr_exp in
+    let b0 = Seq.index (as_seq h0 bp) 0 in
+    let c0 = Seq.index (as_seq h0 cp) 0 in
+    let a0 = b0 +%^ (c0 >>^ d) in
+    let a0, bx = if a0 <^ b0 then mpfr_LIMB_HIGHBIT |^ (a0 >>^ 1ul), I32.(bx +^ 1l) else a0, bx in
+    v a0 * pow2 (I32.v bx - I32.v b.mpfr_exp + U32.v d) = r.limb /\
+    I32.v bx = r.len + I32.v b.mpfr_exp - U32.v d - 64))
+
+let mpfr_add1sp1_gt_branch1_a0_bx_lemma h0 h1 a b c sh d mask =
+    let r = Spec.add_sp (as_reg_fp_ h0 b) (as_reg_fp_ h0 c) in
+    let bp = b.mpfr_d in
+    let cp = c.mpfr_d in
+    let bx = b.mpfr_exp in
+    let b0 = Seq.index (as_seq h0 bp) 0 in
+    let c0 = Seq.index (as_seq h0 cp) 0 in
+    let a0 = b0 +%^ (c0 >>^ d) in
+    let t0 = v b0 + v c0 / pow2 (U32.v d) in
+    //! assert(v a0 = t0 % pow2 64);
+    let a0, bx =
+        if a0 <^ b0 then begin
+	    //! assert(pow2 64 + v a0 = t0);
+	    lemma_div_distr (pow2 64) (v a0) 2;
+	    //! assert(pow2 63 + v a0 / 2 = t0 / pow2 1);
+	    let a0' = mpfr_LIMB_HIGHBIT |^ (a0 >>^ 1ul) in
+	    let bx' = I32.(bx +^ 1l) in
+	    lemma_logor_disjoint mpfr_LIMB_HIGHBIT (a0 >>^ 1ul) 63;
+	    //! assert(v a0' = t0 / pow2 1);
+            lemma_pow2_mod_mod_zero (v b0) (U32.v sh) 1;
+            //! assert(v b0 % pow2 1 = 0);
+            lemma_pow2_mod_mod_zero (v c0) (U32.v sh) (U32.v d + 1);
+            lemma_pow2_mod_div (v c0) (U32.v d + 1) (U32.v d);
+	    //! assert(v c0 / pow2 (U32.v d) % pow2 1 = 0);
+	    lemma_mod_distr_zero (v b0) (v c0 / pow2 (U32.v d)) (pow2 1);
+	    //! assert(t0 / pow2 1 * pow2 1 = t0);
+	    lemma_pow2_div_mul t0 1 1;
+	    //! assert(v a0' * pow2 1 = t0);
+	    a0', bx'
+	end else begin
+	    //! assert(v a0 * pow2 0 = t0);
+	    a0, bx
+	end in
+    //! assert(v a0 * pow2 (I32.v bx - I32.v b.mpfr_exp) = t0);
+    lemma_pow2_mod_mod_zero (v c0) (U32.v sh) (U32.v d);
+    lemma_pow2_div_mul (v c0) (U32.v d) (U32.v d);
+    //! assert(v c0 / pow2 (U32.v d) * pow2 (U32.v d) = v c0);
+    lemma_distr_add_left (v b0) (v c0 / pow2 (U32.v d)) (pow2 (U32.v d));
+    //! assert(t0 * pow2 (U32.v d) = r.limb);
+    lemma_paren_mul_right (v a0) (pow2 (I32.v bx - I32.v b.mpfr_exp)) (pow2 (U32.v d));
+    lemma_pow2_mul (I32.v bx - I32.v b.mpfr_exp) (U32.v d);
+    //! assert(v a0 * pow2 (I32.v bx - I32.v b.mpfr_exp + U32.v d) = r.limb);
+    lemma_pow2_mul_range (v a0) (I32.v bx - I32.v b.mpfr_exp + U32.v d) 64;
+    lemma_bit_length r.limb r.len (I32.v bx - I32.v b.mpfr_exp + U32.v d + 64);
+    //! assert(I32.v bx = r.len + I32.v b.mpfr_exp - U32.v d - 64);
+    ()
+    
+val mpfr_add1sp1_gt_branch1_value_lemma:
+    h0:mem -> h1:mem ->
+    a:mpfr_struct -> b:mpfr_struct -> c:mpfr_struct ->
+    sh:mpfr_reg_prec_t -> d:u32 -> mask:mp_limb_t -> Lemma
+    (requires (mpfr_add1sp1_gt_branch1_precond h0 a b c sh d mask))
+    (ensures  (
+    let p = 64 - U32.v sh in
+    let r = Spec.add_sp (as_reg_fp_ h0 b) (as_reg_fp_ h0 c) in
+    let r = RND.high_mant r p in
+    let bp = b.mpfr_d in
+    let cp = c.mpfr_d in
+    let bx = b.mpfr_exp in
+    let b0 = Seq.index (as_seq h0 bp) 0 in
+    let c0 = Seq.index (as_seq h0 cp) 0 in
+    let a0 = b0 +%^ (c0 >>^ d) in
+    let a0, bx = if a0 <^ b0 then mpfr_LIMB_HIGHBIT |^ (a0 >>^ 1ul), I32.(bx +^ 1l) else a0, bx in
+    let a0 = a0 &^ (lognot mask) in
+    v a0 * pow2 (I32.v bx - I32.v b.mpfr_exp + U32.v d) = r.limb /\
+    I32.v bx = r.len + I32.v b.mpfr_exp - U32.v d - 64))
+
+let mpfr_add1sp1_gt_branch1_value_lemma h0 h1 a b c sh d mask =
+    let p = 64 - U32.v sh in
+    let r = Spec.add_sp (as_reg_fp_ h0 b) (as_reg_fp_ h0 c) in
+    let bp = b.mpfr_d in
+    let cp = c.mpfr_d in
+    let bx = b.mpfr_exp in
+    let b0 = Seq.index (as_seq h0 bp) 0 in
+    let c0 = Seq.index (as_seq h0 cp) 0 in
+    let a0 = b0 +%^ (c0 >>^ d) in
+    let t0 = v b0 + v c0 / pow2 (U32.v d) in
+    let a0, bx = if a0 <^ b0 then mpfr_LIMB_HIGHBIT |^ (a0 >>^ 1ul), I32.(bx +^ 1l) else a0, bx in
+    mpfr_add1sp1_gt_branch1_a0_bx_lemma h0 h1 a b c sh d mask;
+    lemma_pow2_mul_div (v a0) (I32.v bx - I32.v b.mpfr_exp + U32.v d) (r.len - p);
+    //! assert(v a0 / pow2 (64 - p) = r.limb / pow2 (r.len - p));
+    UInt.nth_lemma #64 (UInt.shift_right #64 (v a0) (64 - p)) (UInt.shift_right #64 (UInt.logand (v a0) (UInt.lognot (v mask))) (64 - p));
+    assert(v (a0 &^ lognot mask) / pow2 (64 - p) = r.limb / pow2 (r.len - p));
+    lemma_lognot_mask_mod a0 mask (64 - p);
+    //! assert(v (a0 &^ lognot mask) % pow2 (64 - p) = 0);
+    let a0 = a0 &^ (lognot mask) in
+    lemma_pow2_div_mul (v a0) (64 - p) (r.len - p);
+    //! assert((v a0 / pow2 (64 - p)) * pow2 (r.len - p) = r.limb / pow2 (r.len - p) * pow2 (r.len - p));
+    ()
+
+val mpfr_add1sp1_gt_branch1_rb_lemma:
+    h0:mem -> h1:mem ->
+    a:mpfr_struct -> b:mpfr_struct -> c:mpfr_struct ->
+    sh:mpfr_reg_prec_t -> d:u32 -> mask:mp_limb_t -> Lemma
+    (requires (mpfr_reg_struct_cond h0 b /\ mpfr_reg_struct_cond h0 c /\
+               U32.v a.mpfr_prec < U32.v gmp_NUMB_BITS - 1 /\
+               U32.v a.mpfr_prec = U32.v b.mpfr_prec /\
+               U32.v a.mpfr_prec = U32.v c.mpfr_prec /\
+               U32.v sh = U32.v gmp_NUMB_BITS - U32.v a.mpfr_prec /\
+               U32.v d < U32.v sh /\ v mask = pow2 (U32.v sh) - 1 /\
+               I32.v b.mpfr_exp > I32.v c.mpfr_exp /\
+               (let am = a.mpfr_d in
+               let bm = b.mpfr_d in
+               let cm = c.mpfr_d in
+               live h0 am /\ live h0 bm /\ live h0 cm /\
+	       length am = 1 /\ length bm = 1 /\ length cm = 1)))
+    (ensures  (let p = U32.v a.mpfr_prec in
+               let bp = b.mpfr_d in
+               let cp = c.mpfr_d in
+	       let bx = b.mpfr_exp in
+	       let b0 = Seq.index (as_seq h0 bp) 0 in
+	       let c0 = Seq.index (as_seq h0 cp) 0 in
+	       let a0 = b0 +%^ (c0 >>^ d) in
+	       let a0, bx = if a0 <^ b0 then mpfr_LIMB_HIGHBIT |^ (a0 >>^ 1ul), I32.(bx +^ 1l) else a0, bx in
+	       let rb = a0 &^ (mpfr_LIMB_ONE <<^ U32.(sh -^ 1ul)) in
+	       let res = Spec.add_sp (as_reg_fp_ h0 b) (as_reg_fp_ h0 c) in
+	       v rb <> 0 <==> RND.rb_def res p))
+
+let mpfr_add1sp1_gt_branch1_rb_lemma h0 h1 a b c sh d mask = admit()
+
+val mpfr_add1sp1_gt_branch1_sb_lemma:
+    h0:mem -> h1:mem ->
+    a:mpfr_struct -> b:mpfr_struct -> c:mpfr_struct ->
+    sh:mpfr_reg_prec_t -> d:u32 -> mask:mp_limb_t -> Lemma
+    (requires (mpfr_reg_struct_cond h0 b /\ mpfr_reg_struct_cond h0 c /\
+               U32.v a.mpfr_prec < U32.v gmp_NUMB_BITS - 1 /\
+               U32.v a.mpfr_prec = U32.v b.mpfr_prec /\
+               U32.v a.mpfr_prec = U32.v c.mpfr_prec /\
+               U32.v sh = U32.v gmp_NUMB_BITS - U32.v a.mpfr_prec /\
+               U32.v d < U32.v sh /\ v mask = pow2 (U32.v sh) - 1 /\
+               I32.v b.mpfr_exp > I32.v c.mpfr_exp /\
+               (let am = a.mpfr_d in
+               let bm = b.mpfr_d in
+               let cm = c.mpfr_d in
+               live h0 am /\ live h0 bm /\ live h0 cm /\
+	       length am = 1 /\ length bm = 1 /\ length cm = 1)))
+    (ensures  (let p = U32.v a.mpfr_prec in
+               let bp = b.mpfr_d in
+               let cp = c.mpfr_d in
+	       let bx = b.mpfr_exp in
+	       let b0 = Seq.index (as_seq h0 bp) 0 in
+	       let c0 = Seq.index (as_seq h0 cp) 0 in
+	       let a0 = b0 +%^ (c0 >>^ d) in
+	       let a0, bx = if a0 <^ b0 then mpfr_LIMB_HIGHBIT |^ (a0 >>^ 1ul), I32.(bx +^ 1l) else a0, bx in
+	       let rb = a0 &^ (mpfr_LIMB_ONE <<^ U32.(sh -^ 1ul)) in
+	       let sb = (a0 &^ mask) ^^ rb in
+	       let res = Spec.add_sp (as_reg_fp_ h0 b) (as_reg_fp_ h0 c) in
+	       v sb <> 0 <==> RND.sb_def res p))
+
+let mpfr_add1sp1_gt_branch1_sb_lemma h0 h1 a b c sh d mask = admit()
+
 unfold val mpfr_add1sp1_gt_branch1:
     a:mpfr_struct -> b:mpfr_struct -> c:mpfr_struct ->
     sh:mpfr_reg_prec_t -> d:u32 -> mask:mp_limb_t -> Stack state
-    (requires (fun h -> mpfr_reg_struct_cond h b /\ mpfr_reg_struct_cond h c /\
-                     U32.v a.mpfr_prec < U32.v gmp_NUMB_BITS - 1 /\
-		     U32.v a.mpfr_prec = U32.v b.mpfr_prec /\
-		     U32.v a.mpfr_prec = U32.v c.mpfr_prec /\
-		     U32.v sh = U32.v gmp_NUMB_BITS - U32.v a.mpfr_prec /\
-		     U32.v d < U32.v sh /\ v mask = pow2 (U32.v sh) - 1 /\
-		     I32.v b.mpfr_exp > I32.v c.mpfr_exp /\
-		     (let am = a.mpfr_d in
-		     let bm = b.mpfr_d in
-		     let cm = c.mpfr_d in
-		     live h am /\ live h bm /\ live h cm /\
-		     length am = 1 /\ length bm = 1 /\ length cm = 1)))
-    (ensures  (fun h0 r h1 -> U32.v r.sh = U32.v gmp_NUMB_BITS - U32.v a.mpfr_prec /\
-                           (let am = a.mpfr_d in
-		           let bm = b.mpfr_d in
-		           let cm = c.mpfr_d in
-			   live h1 am /\ live h1 bm /\ live h1 cm /\
-		           modifies_1 am h0 h1)))
+    (requires (fun h -> mpfr_add1sp1_gt_branch1_precond h a b c sh d mask))
+    (ensures  (fun h0 s h1 ->
+    let p = U32.v a.mpfr_prec in
+    U32.v s.sh = U32.v gmp_NUMB_BITS - p /\
+    (let am = a.mpfr_d in
+    let bm = b.mpfr_d in
+    let cm = c.mpfr_d in
+    live h1 am /\ live h1 bm /\ live h1 cm /\
+    modifies_1 am h0 h1 /\
+    (let r = Spec.add_sp (as_reg_fp_ h0 b) (as_reg_fp_ h0 c) in
+    I32.v s.bx >= I32.v b.mpfr_exp /\ I32.v s.bx <= I32.v b.mpfr_exp + 1 /\
+    v (Seq.index (as_seq h1 am) 0) * pow2 (I32.v s.bx - I32.v b.mpfr_exp + U32.v d) = (RND.high_mant r p).limb /\
+    (v s.rb <> 0 <==> RND.rb_def r p) /\
+    (v s.sb <> 0 <==> RND.sb_def r p)))))
 
 let mpfr_add1sp1_gt_branch1 a b c sh d mask =
+    let h0 = ST.get() in
     let ap = a.mpfr_d in
     let bp = b.mpfr_d in
     let cp = c.mpfr_d in
@@ -68,6 +252,10 @@ let mpfr_add1sp1_gt_branch1 a b c sh d mask =
     let rb = a0 &^ (mpfr_LIMB_ONE <<^ U32.(sh -^ 1ul)) in
     let sb = (a0 &^ mask) ^^ rb in
     ap.(0ul) <- a0 &^ (lognot mask);
+    let h1 = ST.get() in
+    mpfr_add1sp1_gt_branch1_value_lemma h0 h1 a b c sh d mask;
+    mpfr_add1sp1_gt_branch1_rb_lemma h0 h1 a b c sh d mask;
+    mpfr_add1sp1_gt_branch1_sb_lemma h0 h1 a b c sh d mask;
     mk_state sh bx rb sb
 
 unfold val mpfr_add1sp1_gt_branch2:
@@ -109,6 +297,7 @@ let mpfr_add1sp1_gt_branch2 a b c sh d mask =
     ap.(0ul) <- a0 &^ (lognot mask);
     mk_state sh bx rb sb
 
+(* TODO: remove abundent inputs *)
 unfold val mpfr_add1sp1_gt_branch3:
     a:mpfr_struct -> b:mpfr_struct -> c:mpfr_struct -> sh:mpfr_reg_prec_t -> Stack state
     (requires (fun h -> mpfr_reg_struct_cond h b /\ mpfr_reg_struct_cond h c /\
